a1.dfy
@@ -1,0 +1,90 @@
+function Power(k: nat): nat {
+  if k == 0 then 1 else 2 * Power(k - 1)
+}
+
+lemma {:axiom} Distrib(a: int, b: int, factor: int)
+  ensures (a+b)*factor == a*factor + b*factor
+{
+}
+
+predicate DivModRel(dividend: int, divisor: int, q: int, r: int)
+{
+  dividend == q*divisor + r && 0 <= r < divisor
+}
+
+/**
+ * A division algorithm using only linear arithmetic and bitwise operations.
+ */
+method DivMod(a: int, b: int) returns (q: int, r: int)
+  requires a >= 0 && b > 0
+  ensures DivModRel(a,b,q,r)
+{
+  assert (b == Power(0)*b && a >= 0);
+  var c := b;
+  assert (0 >= 0 && c == Power(0)*b && a >= 0);
+  var k := 0;
+  assert (k >= 0 && c == Power(k)*b && a >= 0);
+
+  // c is multiplied by 2 until it exceeds our dividend.
+  while c <= a
+    invariant k >= 0 && c == Power(k)*b && a >= 0
+  {
+    assert (k+1 >= 0 && 2*c == Power(k+1)*b && a >= 0);
+    c, k := 2*c, k + 1;
+    assert (k >= 0 && c == Power(k)*b && a >= 0);
+  }
+  assert (c > a && (k >= 0 && c == Power(k)*b && a >= 0));
+  // now, c is greater than a, and is a multiple of 2 and our divisor.
+
+  assert (k >= 0 && c == Power(k)*b && DivModRel(a,c,0,a));
+  q, r := 0, a;
+  // initialise quotient to 0 and remainder to a.
+
+  assert (k >= 0 && c == Power(k)*b && DivModRel(a,c,q,r));
+  while c != b
+    invariant k >= 0 && c == Power(k)*b && DivModRel(a,c,q,r)
+    decreases k
+  {
+    assert k >= 1;
+    assert even: c % 2 == 0 by {
+      assert c == Power(k-1)*b + Power(k-1)*b;
+    }
+
+    calc {
+      (k >= 1 && c == Power(k)*b && DivModRel(a,c,q,r));
+      == { reveal even; }
+      (k-1 >= 0 && c/2 == Power(k-1)*b && a == (q*2)*(c/2)+r && 0 <= r < c);
+    }
+    q, c, k := q*2, c/2, k - 1;
+    assert (k >= 0 && c == Power(k)*b && a == q*c+r && 0 <= r < c+c);
+
+    assert (
+      (r >= c ==> k >= 0 && c == Power(k)*b && a == q*c + r && r < c+c)
+      && 
+      (r < c  ==> k >= 0 && c == Power(k)*b && a == q*c+r && 0 <= r)
+    );
+
+    assert (
+      if r >= c 
+      then (k >= 0 && c == Power(k)*b && a == q*c + r && 0 <= r-c < c)
+      else (k >= 0 && c == Power(k)*b && DivModRel(a,c,q,r)));
+
+    if r >= c {
+      calc {
+        (k >= 0 && c == Power(k)*b && a == q*c + r && 0 <= r-c < c);
+        ==
+        (k >= 0 && c == Power(k)*b && a == ((q)*c + c) + (r-c) && 0 <= r-c < c);
+        ==
+        (k >= 0 && c == Power(k)*b && DivModRel(a,c,q+1,r-c));
+      }
+      q, r := q + 1, r - c;
+      assert (k >= 0 && c == Power(k)*b && DivModRel(a,c,q,r));
+    }
+    assert (k >= 0 && c == Power(k)*b && DivModRel(a,c,q,r));
+  }
+  calc {
+    c == b && (k >= 0 && c == Power(k)*b && DivModRel(a,c,q,r)); 
+    ==
+    DivModRel(a,b,q,r);
+  }
+}
