a2.dfy
@@ -1,0 +1,83 @@
+ghost function Count(lo: nat, hi: nat, s:seq<int>):int
+  requires lo <= hi <= |s|
+  decreases hi - lo
+{
+  if lo == hi then 0
+  else if s[hi-1]%2 == 0 then 1 + Count(lo, hi-1, s) else Count(lo, hi-1, s)
+}
+
+method PreCompute(a: array<int>, b: array<int>)
+  requires a.Length == b.Length
+  requires a != b
+  modifies b
+
+  ensures forall i :: 0 <= i < b.Length ==> b[i] == Count(0,i+1,a[..])
+{
+  ComputeCount(a,b,0);
+}
+
+method ComputeCount(a: array<int>, b: array<int>, n: nat)
+  requires a.Length == b.Length
+  requires a != b
+  modifies b
+
+  requires n <= a.Length
+  decreases a.Length - n
+
+  requires forall i :: 0 <= i < n ==> b[i] == Count(0,i+1,a[..])
+  ensures forall i :: 0 <= i < a.Length ==> b[i] == Count(0,i+1,a[..])
+{
+  if n == a.Length {
+    return;
+  }
+  var d := 1 - a[n] % 2;
+  b[n] := d + (if n == 0 then 0 else b[n-1]);
+  ComputeCount(a, b, n+1);
+}
+
+lemma CountOfSlice(lo: nat, hi: nat, s: seq<int>)
+  requires lo <= hi <= |s|
+  ensures Count(lo,hi,s) == Count(0,hi,s) - Count(0,lo,s)
+{}
+
+method Evens(a: array<int>) returns (c: array2<int>)
+  ensures fresh(c)
+  ensures a.Length == c.Length0 == c.Length1
+  ensures forall i,j :: 0 <= i <= j < a.Length ==>
+                          c[i,j] == Count(i,j+1,a[..])
+
+{
+  c := new int[a.Length,a.Length];
+
+  var b := new int[a.Length];
+  PreCompute(a,b);
+
+  for ii := 0 to a.Length
+    invariant forall i :: 0 <= i < b.Length ==> b[i] == Count(0,i+1,a[..])
+    invariant forall i,j :: 0 <= i <= j < a.Length && i < ii ==> c[i,j] == Count(i,j+1,a[..])
+  {
+    for jj := ii to a.Length
+      invariant forall i :: 0 <= i < b.Length ==> b[i] == Count(0,i+1,a[..])
+      invariant forall i,j :: 0 <= i <= j < a.Length && i < ii ==> c[i,j] == Count(i,j+1,a[..])
+      invariant forall i,j :: 0 <= i <= j < jj && i == ii ==> c[i,j] == Count(i,j+1,a[..])
+    {
+      CountOfSlice(ii,jj+1,a[..]); 
+      c[ii,jj] := b[jj] - if ii > 0 then b[ii-1] else 0;
+    }
+  }
+}
+
+method PreComputeLoop(a: array<int>, b: array<int>)
+  requires a.Length == b.Length
+  requires a != b
+  modifies b
+
+  ensures forall i :: 0 <= i < b.Length ==> b[i] == Count(0,i+1,a[..])
+{
+  for n := 0 to a.Length
+    invariant forall i :: 0 <= i < n ==> b[i] == Count(0,i+1,a[..])
+  {
+    var d := 1 - a[n] % 2;
+    b[n] := d + (if n == 0 then 0 else b[n-1]);
+  }
+}
