params.dfy
@@ -1,0 +1,24 @@
+function Power(k: nat): nat {
+if k == 0 then 1 else 2 * Power(k - 1)
+}
+method DivMod(a: int, b: int) returns (q: int, r: int)
+ requires a >= 0 && b > 0
+ ensures a == q*b + r && 0 <= r < b
+{
+ var c := b;
+ var k := 0;
+ while c <= a
+ invariant k >= 0 && c == Power(k)*b && a >= 0
+ {
+ c, k := 2*c, k + 1;
+ }
+ q, r := 0, a;
+ while c != b 
+ invariant k >= 0 && c == Power(k)*b && a == q*c + r && 0 <= r < c
+ {
+ q, c, k := q*2, c/2, k - 1;
+ if r >= c {
+ q, r := q + 1, r - c;
+ }
+ }
+}
