project.dfy
@@ -1,0 +1,105 @@
+function Project<T(==)>(xs: seq<T>, key: T): seq<T>
+{
+  if xs == [] then [] 
+  else if xs[0] == key then [key] + Project(xs[1..],key)
+  else Project(xs[1..],key)
+}
+
+lemma MultisetMultiplicity<T>(ms: seq<T>, x: T)
+requires ms != []
+requires ms[0] != x
+ensures multiset(ms)[x] == multiset(ms[1..])[x]
+{
+  assert ms == [ms[0]] + ms[1..];
+}
+
+// lemma ProjectHomo<T>(xs: seq<T>, ys: seq<T>, key: T)
+//   ensures Project(xs+ys,key) == Project(xs,key) + Project(ys,key)
+// {
+//   if xs == [] {
+//     assert xs+ys == ys;
+//   } else if ys == [] {
+//     assert xs+ys == xs;
+//   } else {
+
+//   }
+// }
+
+lemma SeqAppendFront<T>(front: seq<T>, xs: seq<T>, ys: seq<T>)
+  requires front + xs == front + ys 
+  ensures xs == ys
+{
+  if xs == [] {}
+  else if ys == [] {}
+  else if |xs| != |ys| {}
+  else if xs != ys {
+    var i :| 0 <= i < |xs| && xs[i] != ys[i];
+    assert (front + xs)[i+|front|] == xs[i]; 
+  }
+}
+
+lemma ProjectCardinality<T>(xs: seq<T>, key: T)
+  ensures |Project(xs,key)| == multiset(xs)[key] 
+{
+  if xs == [] {}
+  else if xs[0] != key {
+    assert Project(xs,key) == Project(xs[1..],key);
+    assert xs == [xs[0]] + xs[1..];
+    assert multiset(xs)[key] == multiset(xs[1..])[key];
+    ProjectCardinality(xs[1..], key);
+  }
+}
+
+
+lemma ProjectCardinalityEqual<T>(xs: seq<T>, ys: seq<T>, key: T)
+  requires |Project(xs,key)| == |Project(ys,key)|
+  ensures multiset(xs)[key] == multiset(ys)[key]
+{
+  ProjectCardinality(xs,key);
+  ProjectCardinality(ys,key);
+}
+
+lemma ProjectToMultiset<T>(xs: seq<T>, ys: seq<T>)
+  requires forall x :: x in xs || x in ys ==> |Project(xs,x)| == |Project(ys,x)|
+  ensures multiset(xs) == multiset(ys)
+  decreases |ys| < |xs|
+{
+  if xs == [] {
+    if ys != [] {
+      assert Project(ys,ys[0]) != [];
+    }
+  } else if ys == [] {
+    ProjectToMultiset(ys,xs);
+  } else if multiset(xs) != multiset(ys) {
+    var diff :| multiset(xs)[diff] != multiset(ys)[diff];
+    ProjectCardinality(xs,diff);
+    ProjectCardinality(ys,diff);
+  }
+}
+
+lemma MultisetToProject<T>(xs: seq<T>, ys: seq<T>)
+  requires multiset(xs) == multiset(ys)
+  ensures forall x :: x in xs || x in ys ==> |Project(xs,x)| == |Project(ys,x)|
+{
+  if xs == [] {} 
+  else if ys == [] {}
+  else {
+    forall x | x in xs || x in ys
+      ensures |Project(xs,x)| == |Project(ys,x)|
+    {
+      assert multiset(xs)[x] == multiset(ys)[x];
+      ProjectCardinality(xs,x);
+      ProjectCardinality(ys,x);
+    }
+  }
+}
+
+lemma MultisetCardinalityEqual<T>(xs: seq<T>, ys: seq<T>)
+  requires |multiset(xs)| == |multiset(ys)|
+  ensures |xs| == |ys| 
+{}
+
+lemma StableImpliesUnstable<T>(xs: seq<T>, ys: seq<T>)
+  requires forall x :: x in xs || x in ys ==> Project(xs,x) == Project(ys,x)
+  ensures forall x :: x in xs || x in ys ==> |Project(xs,x)| == |Project(ys,x)|
+{}
