spec2.dfy
@@ -1,0 +1,287 @@
+datatype L = Low | High
+
+predicate leq(l1:L,l2:L) {
+    (l1 == Low || l2 == High)
+}
+
+// upper bound on l1 and l2
+function join(l1:L,l2:L):L {
+    if leq(l1,l2) then l2 else l1
+}
+// lower bound on l1 and l2
+function meet(l1:L,l2:L):L {
+    if leq(l1,l2) then l1 else l2
+}
+
+lemma partialorder(l1:L,l2:L,l3:L)
+ensures leq(l1,l1) // reflexivity
+ensures leq(l1,l2) && leq(l2,l1) ==> l1 == l2 // antisymmetry
+ensures leq(l1,l2) && leq(l2,l3) ==> leq(l1,l3) // transitivity
+{}
+
+lemma joinLemma(l1:L,l2:L,l3:L)
+ensures leq(l1,join(l1,l2)) && leq(l2,join(l1,l2))
+ensures leq(l1,l3) && leq(l2,l3) ==> leq(join(l1,l2),l3)
+ensures join(l1,l2) == join(l2,l1)
+{}
+
+lemma meetLemma(l1:L,l2:L,l3:L)
+ensures leq(meet(l1,l2),l1) && leq(meet(l1,l2),l2)
+ensures leq(l3,l1) && leq(l3,l2) ==> leq(l3,meet(l1,l2))
+ensures meet(l1,l2) == meet(l2,l1)
+{}
+
+
+datatype Frame<T> = Frame(x: T, z: T, secret: T, leak: T)
+datatype Val<L, T> = V(v: T, gamma: L)
+// type Vars = Frame<Val<L, int>> // mapping of variable to their values.
+
+function lift<T>(v1: Val<L,T>, v2: Val<L,T>, f: (T,T) --> T): Val<L,T>
+    requires f.requires(v1.v, v2.v)
+    ensures leq(v1.gamma,lift(v1,v2,f).gamma)
+    ensures leq(v2.gamma,lift(v1,v2,f).gamma)
+{
+    V(f(v1.v, v2.v), join(v1.gamma, v2.gamma))
+}
+
+function pure<T>(t: T): Val<L,T>
+{
+    V(t,Low)
+}
+
+
+
+type V = Val<L,int>
+type Vars = Frame<V>
+datatype Idx = X | Z | SECRET | LEAK
+class Spec {
+    var Vars: Vars;
+    var SVars: Vars;
+    var Qspec: bool;
+    const VARS := {X, Z, SECRET, LEAK};
+
+    constructor()
+        ensures Secure()
+    {
+        Vars := Frame(V(0,Low), V(0,Low), V(10,High), V(0,Low));
+        // SVars := Vars;
+    }
+
+    // levels are to be calculated from the concrete "base" Vars.
+    function Levels(): Frame<L>
+        reads this
+    {
+        Frame(High, Low, High, Low)
+    }
+
+    predicate Secure(globals: Vars := Vars)
+        reads this
+        ensures X in VARS
+        ensures Z in VARS
+        ensures SECRET in VARS 
+        ensures LEAK in VARS
+    {
+        (forall v | v in VARS :: leq(Read(v).gamma, Read(v, globals).gamma))
+        // && leq(Read(LEAK).gamma, Level(LEAK))
+    }
+
+    function Level(index: Idx): L
+        reads this
+    {
+        match index case X => Levels().x case Z => Levels().z case SECRET => Levels().secret case LEAK => Levels().leak
+    }
+
+    function Read(index: Idx, vars: Vars := Vars): V
+        reads this
+    {
+        match index case X => vars.x case Z => vars.z case SECRET => vars.secret case LEAK => vars.leak
+    }
+
+    method Store(index: Idx, v: V)
+        modifies this
+        requires leq(v.gamma, Level(index))
+
+        ensures Vars == match index case X => old(Vars).(x := v) case Z => old(Vars).(z := v) case SECRET => old(Vars).(secret := v) case leak => old(Vars).(leak := v)
+        // note: does not perform "secure update" check on controlled variables.
+        // Secure() should be asserted after invoking this.
+    {
+        Vars := match index case X => (Vars).(x := v) case Z => (Vars).(z := v) case SECRET => (Vars).(secret := v) case LEAK => Vars.(leak := v);
+    }
+
+    static function add(x: int, y: int): int
+    {
+        x + y
+    }
+
+    method nospec()
+        modifies this 
+        requires Secure()
+        requires Vars.z.v == 0
+        // requires Vars.leak.gamma == Low
+        ensures Secure()
+    {
+        Rely(R_nospec);
+        label 1:
+        Store(X, V(-1, Low));
+        assert Guar@1(G_nospec);
+        assert Secure();
+
+        Rely(R_nospec);
+        label 2:
+        if (Read(Z).v == 0)
+        {
+            assert Guar@2(G_nospec);
+            assert Secure();
+
+            Rely(R_nospec);
+            label 3: var x := Read(X);
+            assert Guar@3(G_nospec);
+            assert Secure();
+
+            Rely(R_nospec);
+            label 4: Store(LEAK, x);
+            assert Guar@4(G_nospec);
+            assert Secure();
+        }
+        assert Guar@2(G_nospec);
+        assert Secure();
+    }
+
+    method spec()
+        modifies this 
+        requires Secure()
+        requires Vars.z.v == 0
+        // requires Vars.leak.gamma == Low
+        ensures Secure()
+    {
+        Rely(R_nospec);
+        label 1:
+        Store(X, V(-1, Low));
+        assert Guar@1(G_nospec);
+        assert Secure();
+
+        Rely(R_nospec);
+        label 2:
+        // if (Read(Z).v == 0)
+        if (true)
+        {
+            assert Guar@2(G_nospec);
+            assert Secure();
+
+            Rely(R_nospec);
+            label 3: var x := Read(X);
+            assert Guar@3(G_nospec);
+            assert Secure();
+
+            Rely(R_nospec);
+            label 4: Store(LEAK, x);
+            assert Guar@4(G_nospec);
+            assert Secure();
+        }
+        assert Guar@2(G_nospec);
+        assert Secure();
+    }
+
+
+    method R_reflexive()
+        ensures R_nospec(Vars)
+    {}
+
+    predicate R_nospec(old_vars: Vars)
+        reads this
+    {
+        (old_vars.z.v == 0 ==> old_vars.z == Vars.z && leq(Vars.x.gamma, old_vars.x.gamma))
+        && Vars.leak == old_vars.leak
+        && leq(Vars.z.gamma, old_vars.z.gamma)
+    }
+
+    predicate G_nospec(prev: Vars)
+        reads this 
+    {
+        true
+    }
+
+    method test()
+        modifies this
+        requires Secure()
+    {
+        Store(SECRET, V(1, Low));
+
+        // var e := lift(Vars.secret, pure(10), add);
+        // assert leq(e.gamma, Levels()[x]);
+
+        // Vars := Vars.x := e;
+        // Vars, Gammas := Vars.(x := e), Gammas.(x := Gamma_e);
+        // assert Secure();
+    }
+
+    // method sync_write()
+    //     modifies this
+    //     requires Secure()
+    //     requires Vars.z.v % 2 == 0
+
+    //     ensures Secure()
+    // {
+    //     // sync_write_R();
+    //     Rely(public_read_G);
+
+    //     label 1: var z' := lift(Read(Z), pure(1), add);
+    //     Store(Z, z');
+    //     assert Guar@1(sync_write_G);
+    //     assert Secure();
+
+    //     Rely(public_read_G);
+    //     // sync_write_R();
+    //     // label l:
+    //     // modify this;
+    //     // assume Valid() && public_read_G(Vars@l);
+
+    //     label 2: var x' := Vars.secret;
+    //     Store(X, x');
+    //     assert Guar@2(sync_write_G);
+    //     assert Secure();
+
+    //     Rely(public_read_G);
+
+    //     label 3: var x'' := pure(0);
+    //     Store(X, x'');
+    //     assert Guar@3(sync_write_G);
+    //     assert Secure();
+
+    //     Rely(public_read_G);
+
+    //     label 4: var z'' := lift(Vars.z, pure(1), add);
+    //     Store(Z, z'');
+    //     assert Guar@4(sync_write_G);
+    //     assert Secure();
+
+    //     Rely(public_read_G);
+    // }
+
+    method Rely(rely: (Vars) ~> bool)
+        modifies this
+        requires rely.requires(Vars)
+        ensures rely.requires(old(Vars))
+        ensures rely(old(Vars))
+
+    twostate predicate Guar(guar: (Vars) ~> bool)
+        reads this, guar.reads
+        requires guar.requires(old(Vars))
+    {
+        guar(old(Vars))
+    }
+
+    predicate public_read_G(old_vars: Vars)
+        reads this
+    {
+        // true
+        leq(Vars.x.gamma, (old_vars.x.gamma))
+        && Vars.z == old_vars.z
+    }
+
+    predicate sync_write_G(Old: Vars)
+        reads this
+    {
+        Vars.z.v >= Old.z.v
+    }
+}
